

Using rules of expectations to re-express the variance

Let $\mu = E[X]$. The variance of X is

$$\begin{aligned} V &= E[(X - \mu)^2] && \text{(by Eqn. ??)} \\ &= E[X^2 - 2\mu X + \mu^2] \end{aligned}$$

Using rules of expectations to re-express the variance

Let $\mu = E[X]$. The variance of X is

$$V = E[(X - \mu)^2] \quad (\text{by Eqn. ??})$$

$$= E[X^2 - 2\mu X + \mu^2]$$

$$= E[X^2] - E[2\mu X] + E[\mu^2] \quad (\text{by Eqn. ??})$$

$$= E[X^2] - E[2\mu X] + \mu^2 \quad (\text{by Eqn. ??})$$

Using rules of expectations to re-express the variance

Let $\mu = E[X]$. The variance of X is

$$V = E[(X - \mu)^2] \quad (\text{by Eqn. ??})$$

$$= E[X^2 - 2\mu X + \mu^2]$$

$$= E[X^2] - E[2\mu X] + E[\mu^2] \quad (\text{by Eqn. ??})$$

$$= E[X^2] - E[2\mu X] + \mu^2 \quad (\text{by Eqn. ??})$$

$$= E[X^2] - 2\mu E[X] + \mu^2 \quad (\text{by Eqn. ??})$$

$$= E[X^2] - 2\mu^2 + \mu^2 \quad (\text{by definition of } \mu)$$

$$= E[X^2] - \mu^2$$